\section{Suppose $f:I \to \R$ where $I$ is an open interval containing $a$.
    Suppose further that $f$ is $n$ times differentiable at $a$ 
    and let $p_n$ be the $n$th Taylor polynomial for $f$ at $a$.
    Apply \lhopital's rule $n-1$ times to show that
    \[
        \bm{\lim_{x\to a}\frac{f(x) - p_n(x)}{(x-a)^n} = 0}
    \]
}
    % % Attempt 3, turns out i was using the wrong def for \lhopital, and question has typo (?).
    Let $g(x) = (f(x) - p_n(x))$.
    Let $h(x) = (x-a)^n$.
    As $\lall k, 1 < k \leq n, h^{(k)}(x)$ is non-zero for all deleted nhds of $a$,
    we can apply \lhopital's rule $n$ times.
    So $g^{(n)} = f^{(n)}(x) - p_n^{(n)}(x)$,
    and $h^{(n)} = n!$.

    \begin{align*}
        \lim_{x\to a}\frac{f(x) - p_n(x)}{(x-a)^n}
        &= \lim_{x\to a}\frac{f^{(n)}(x) - p_n^{(n)}(x)}{n!} \\
        &= \lim_{x\to a}\frac{f^{(n)}(a) - p_n^{(n)}(a)}{n!} 
            \text{ (TODO, are $f^{(n)}, p^{(n)}_n$ are continuous?)} \\
        &= \lim_{x\to a}\frac{0}{n!} \\
        &= 0
    \end{align*}


    % % Attempet 2
    % % Doesn't work, c depends of x
    % Let $\e > 0$.
    % By Taylor's Theorem, 
    % $\lis c$ such that 
    % $f(x) = p_n(x) + \frac{f^{(n+1)}(c)}{(n+1)!} (x-x_0)^{n+1}$.
    % Choose $\delta = \e \abs{\frac{f^{(n+1)}(c)}{(n+1)!}}^{-1}$.
    % \footnote{If $\frac{f^{(n+1)}(c)}{(n+1)!} = 0$, then $\delta$ can be anything, and the proof is trivial.}
    % Let $\abs{x - a} < \delta$.
    % \begin{align*}
    %     \abs{\frac{f(x) - p_n(x)}{(x-a)^n} - 0}
    %     &= \abs{\frac{(p_n(x) + \frac{f^{(n+1)}(c)}{(n+1)!} (x-a)^{n+1}) - p_n(x)}{(x-a)^n}} \\
    %     &= \abs{\frac{f^{(n+1)}(c)}{(n+1)!} (x-a)} \\
    %     &= \abs{\frac{f^{(n+1)}(c)}{(n+1)!}} \abs{x-a} \\
    %     &< \abs{\frac{f^{(n+1)}(c)}{(n+1)!}} \e \abs{\frac{f^{(n+1)}(c)}{(n+1)!}}^{-1} \\
    %     &= \e
    % \end{align*}
    

    % % Attempt 1
    % Let $g(x) = a(x) (f(x) - p_n(x))$.
    % Let $h(x) = a(x) (x-a)^n$.
    % So $h'(x) = a'(x) (x-a)^n + n (x-a)^{n-1} a(x)$.

    % $a(x)$ could be $(x-a)^{1-n}$.
    % $a'(x)$ would be $(-n+1)(x-a)^{-n}$.


    % So $g^{(n-1)} = f^{(n-1)}(x) - p_n^{(n-1)}(x)$,
    % and $h^{(n-1)} = n! (x - a)$.
    % \begin{align*}
    %     test
    % \end{align*}