\section{Suppose that $f,g,h$ are functions from $\R$ to $\R$.}
    \subsection{Show that there does not exist $f,g$ satisfying $f(x) + g(y) = xy$ for all $x,y \in \R$.}
        Let $f, g : \R \to \R$.
        Suppose there exists functions $f,g$ such that $f(x) + g(y) = xy$.
        Lets choose $x = 0$, then that means $f(0) + g(y) = 0$. 
        So $f(0) = -g(y)$ for all $y$.
        Therefore $g(y)$ is a constant.
        So we have $f(x) + c = xy, c\in \R$.
        Now choose $x = 1, y = 1$.
        Then $f(1) + c = 1$.
        Now choose $x = 1, y = 2$.
        Then $f(1) + c = 2$.
        Which is a contradiction.
        Therefore there does not exist functions $f, g$ such that $f(x) + g(y) = xy$.

    \subsection{Show that there does not exist $f,g$ satisfying $f(x)g(y) = x+y$ for all $x,y \in \R$.}
        Let $f, g : \R \to \R$.
        Suppose there exists functions $f,g$ such that $f(x)g(y) = x + y$.
        Lets choose $x = 0$.
        Then $f(0)g(y) = y$.
        If $f(0) = 0$ then we have an immediate contradiction,
        as $0 = y, \forall y \in \R$.
        Therefore $f(0) \neq 0$.
        Therefore $g(y) = y / f(0)$.
        Let $c = f(0) \neq 0, c \in \R$.
        Substitute that back into the original equation to get
        $f(x) y / c= x + y$.
        Or $f(x) y = c(x + y)$.
        Now choose $y = 0, x \in \R$.
        Then $0 = c(x)$.
        And because we know $c \neq 0$,
        so $x = 0, \forall x \in \R$.
        Which is a contradiction.
        Therefore there does not exist functions $f, g$ such that $f(x)g(y) = x + y$.
        

    \subsection{Show that there does not exist three functions $f,g,h$ which satisfy
        \[f(x) + g(y) + h(z) = xyz
            \]
        for all $x,y,z \in \R$.}

        Let $f, g, h : \R \to \R$.
        Suppose there exists functions $f,g,h$ such that $f(x) + g(y) + h(z) = xyz$.
        Lets choose $x = 0, y = 0$, then that means $f(0) + g(0) + h(z) = 0$. 
        That means $h(z)$ is a constant for all $z \in \R$.
        So now we have $f(x) + g(y) + c = xyz, c \in \R$.
        Now choose $x = y = z = 1$. 
        Then $f(1) + g(1) + c = 1$.
        And now, choose $ x = y = 1, z = 2$.
        Then $f(1) + g(1) + c = 2$.
        Which is a contradiction.
        Therefore there do not exist functions $f,g,h$ such that $f(x) + g(y) + h(z) = xyz$.